Created explicit pointer-type tags for the unstructured phases

10FlatMemory/FlatMemory.thy
@@ -1,20 +1,20 @@
 theory FlatMemory
-  imports "../07ByteCode/ByteCode" "../08HeapMemory/Heap"
+  imports "../07ByteCode/ByteCode" "../08HeapMemory/Heap" PointerTag
 begin
 
 text \<open>The chained memory stage is quite low-level, but it still possesses some structured data: 
 pairs in the stack and the environment heap, and tagged closure-values in the value heap. We now 
 reduce all of these to contiguous series of numbers. The pairs are just listed, first component 
-first; the closures are flattened to sequences of data. A \<open>Const\<^sub>v n\<close> value becomes \<open>[1, n, 0]\<close>; a 
-\<open>Lam\<^sub>v p\<^sub>\<Delta> p\<^sub>\<C>\<close> becomes \<open>[0, p\<^sub>\<Delta>, p\<^sub>\<C>]\<close>. The first element is a tag indicating what sort of value we have;
-intuitively, we shouldn't need it (we could just stop testing the tag in \<open>ev\<^sub>f_apply\<close> and \<open>ev\<^sub>f_jump\<close>)
-but in fact it will be necessary for some of the future stages. Specifically, we need to know when a
-number is a code pointer to be treated differently than data or data pointers, and that requires 
-knowing when a block of data is a lambda-value. (The padding 0 on the numerical values is just to 
-keep all values the same size, greatly easing some of the proofs.)\<close>
+first; the closures are flattened to sequences of data. A \<open>Const\<^sub>v n\<close> value becomes \<open>[n, 0]\<close>; a 
+\<open>Lam\<^sub>v p\<^sub>\<Delta> p\<^sub>\<C>\<close> becomes \<open>[p\<^sub>\<Delta>, p\<^sub>\<C>]\<close>. We tag the code pointers because we need to recognize them later, 
+when we move to assembly code and alter all the codeblock addresses; besides that, in losing the 
+tags on values, we have now discarded our last scrap of type-safety. The \<open>ev\<^sub>f_apply\<close> and \<open>ev\<^sub>f_jump\<close> 
+operations assume they've been given a function-closure, but no longer have a way of checking it. 
+(The padding 0 on the numerical values is just to keep all values the same size, greatly easing some 
+of the proofs.)\<close>
 
 datatype state\<^sub>f = 
-  S\<^sub>f "nat heap" "ptr heap" "ptr list" "nat list"
+  S\<^sub>f "(pointer_tag \<times> nat) heap" "ptr heap" "ptr list" "nat list"
 
 fun flat_lookup :: "ptr heap \<Rightarrow> ptr \<Rightarrow> nat \<rightharpoonup> ptr" where
   "flat_lookup h 0 x = None"
@@ -26,20 +26,22 @@ fun flat_lookup :: "ptr heap \<Rightarrow> ptr \<Rightarrow> nat \<rightharpoonu
 inductive eval\<^sub>f :: "code\<^sub>b list \<Rightarrow> state\<^sub>f \<Rightarrow> state\<^sub>f \<Rightarrow> bool" (infix "\<tturnstile> _ \<leadsto>\<^sub>f" 50) where
   ev\<^sub>f_lookup [simp]: "lookup \<C> p\<^sub>\<C> = Some (Lookup\<^sub>b x) \<Longrightarrow> flat_lookup \<Delta> p\<^sub>\<Delta> x = Some v \<Longrightarrow> 
     \<C> \<tturnstile> S\<^sub>f h \<Delta> \<V> (Suc p\<^sub>\<C> # p\<^sub>\<Delta> # s) \<leadsto>\<^sub>f S\<^sub>f h \<Delta> (v # \<V>) (p\<^sub>\<C> # p\<^sub>\<Delta> # s)"
-| ev\<^sub>f_pushcon [simp]: "lookup \<C> p\<^sub>\<C> = Some (PushCon\<^sub>b n) \<Longrightarrow> halloc_list h [1, n, 0] = (h', v) \<Longrightarrow>
-    \<C> \<tturnstile> S\<^sub>f h \<Delta> \<V> (Suc p\<^sub>\<C> # p\<^sub>\<Delta> # s) \<leadsto>\<^sub>f S\<^sub>f h' \<Delta> (v # \<V>) (p\<^sub>\<C> # p\<^sub>\<Delta> # s)"
-| ev\<^sub>f_pushlam [simp]: "lookup \<C> p\<^sub>\<C> = Some (PushLam\<^sub>b p\<^sub>\<C>') \<Longrightarrow> halloc_list h [0, p\<^sub>\<Delta>, p\<^sub>\<C>'] = (h', v) \<Longrightarrow> 
-    \<C> \<tturnstile> S\<^sub>f h \<Delta> \<V> (Suc p\<^sub>\<C> # p\<^sub>\<Delta> # s) \<leadsto>\<^sub>f S\<^sub>f h' \<Delta> (v # \<V>) (p\<^sub>\<C> # p\<^sub>\<Delta> # s)"
-| ev\<^sub>f_apply [simp]: "lookup \<C> p\<^sub>\<C> = Some Apply\<^sub>b \<Longrightarrow> hlookup h v\<^sub>2 = 0 \<Longrightarrow> 
-    halloc_list \<Delta> [v\<^sub>1, hlookup h (Suc v\<^sub>2)] = (\<Delta>', p\<^sub>\<Delta>') \<Longrightarrow> 
+| ev\<^sub>f_pushcon [simp]: "lookup \<C> p\<^sub>\<C> = Some (PushCon\<^sub>b n) \<Longrightarrow> 
+    halloc_list h [(PConst, 1), (PConst, n), (PConst, 0)] = (h', v) \<Longrightarrow>
+      \<C> \<tturnstile> S\<^sub>f h \<Delta> \<V> (Suc p\<^sub>\<C> # p\<^sub>\<Delta> # s) \<leadsto>\<^sub>f S\<^sub>f h' \<Delta> (v # \<V>) (p\<^sub>\<C> # p\<^sub>\<Delta> # s)"
+| ev\<^sub>f_pushlam [simp]: "lookup \<C> p\<^sub>\<C> = Some (PushLam\<^sub>b p\<^sub>\<C>') \<Longrightarrow> 
+    halloc_list h [(PConst, 0), (PEnv, p\<^sub>\<Delta>), (PCode, p\<^sub>\<C>')] = (h', v) \<Longrightarrow> 
+      \<C> \<tturnstile> S\<^sub>f h \<Delta> \<V> (Suc p\<^sub>\<C> # p\<^sub>\<Delta> # s) \<leadsto>\<^sub>f S\<^sub>f h' \<Delta> (v # \<V>) (p\<^sub>\<C> # p\<^sub>\<Delta> # s)"
+| ev\<^sub>f_apply [simp]: "lookup \<C> p\<^sub>\<C> = Some Apply\<^sub>b \<Longrightarrow> snd (hlookup h v\<^sub>2) = 0 \<Longrightarrow> 
+    halloc_list \<Delta> [v\<^sub>1, snd (hlookup h (Suc v\<^sub>2))] = (\<Delta>', p\<^sub>\<Delta>') \<Longrightarrow> 
     \<C> \<tturnstile> S\<^sub>f h \<Delta> (v\<^sub>1 # v\<^sub>2 # \<V>) (Suc p\<^sub>\<C> # p\<^sub>\<Delta> # s) \<leadsto>\<^sub>f 
-      S\<^sub>f h \<Delta>' \<V> (hlookup h (Suc (Suc v\<^sub>2)) # Suc (Suc p\<^sub>\<Delta>') # p\<^sub>\<C> # p\<^sub>\<Delta> # s)"
+      S\<^sub>f h \<Delta>' \<V> (snd (hlookup h (Suc (Suc v\<^sub>2))) # Suc (Suc p\<^sub>\<Delta>') # p\<^sub>\<C> # p\<^sub>\<Delta> # s)"
 | ev\<^sub>f_return [simp]: "lookup \<C> p\<^sub>\<C> = Some Return\<^sub>b \<Longrightarrow> 
     \<C> \<tturnstile> S\<^sub>f h \<Delta> \<V> (Suc p\<^sub>\<C> # p\<^sub>\<Delta> # s) \<leadsto>\<^sub>f S\<^sub>f h \<Delta> \<V> s"
-| ev\<^sub>f_jump [simp]: "lookup \<C> p\<^sub>\<C> = Some Jump\<^sub>b \<Longrightarrow> hlookup h v\<^sub>2 = 0 \<Longrightarrow> 
-    halloc_list \<Delta> [v\<^sub>1, hlookup h (Suc v\<^sub>2)] = (\<Delta>', p\<^sub>\<Delta>') \<Longrightarrow> 
+| ev\<^sub>f_jump [simp]: "lookup \<C> p\<^sub>\<C> = Some Jump\<^sub>b \<Longrightarrow> snd (hlookup h v\<^sub>2) = 0 \<Longrightarrow> 
+    halloc_list \<Delta> [v\<^sub>1, snd (hlookup h (Suc v\<^sub>2))] = (\<Delta>', p\<^sub>\<Delta>') \<Longrightarrow> 
       \<C> \<tturnstile> S\<^sub>f h \<Delta> (v\<^sub>1 # v\<^sub>2 # \<V>) (Suc p\<^sub>\<C> # p\<^sub>\<Delta> # s) \<leadsto>\<^sub>f 
-        S\<^sub>f h \<Delta>' \<V> (hlookup h (Suc (Suc v\<^sub>2)) # Suc (Suc p\<^sub>\<Delta>') # s)"
+        S\<^sub>f h \<Delta>' \<V> (snd (hlookup h (Suc (Suc v\<^sub>2))) # Suc (Suc p\<^sub>\<Delta>') # s)"
 
 theorem determinismf: "\<C> \<tturnstile> \<Sigma> \<leadsto>\<^sub>f \<Sigma>' \<Longrightarrow> \<C> \<tturnstile> \<Sigma> \<leadsto>\<^sub>f \<Sigma>'' \<Longrightarrow> \<Sigma>' = \<Sigma>''"
 proof (induction \<Sigma> \<Sigma>' rule: eval\<^sub>f.induct)
