10FlatMemory/PointerTag.thy
@@ -1,0 +1,15 @@
+theory PointerTag
+  imports Main
+begin
+
+section \<open>Flat Memory\<close>
+
+text \<open>We declare some tags for the various sorts of pointers we use; they live in a separate file so 
+they can be reused by later stages.\<close>
+
+datatype pointer_tag = 
+  PConst
+  | PEnv
+  | PCode
+
+end
